examples/iso_dh/README.md
@@ -1,0 +1,48 @@
+# Formal Security Analysis of the ISO-DH Protocol
+
+This folder contains a formal security analysis
+of the Diffie-Hellman key exchange protocol with 
+digital signatures based on the [ISO/IEC 9798-3:2019(E)](https://www.iso.org/standard/67115.html) 
+standard. In this analysis, we prove the following 
+properties of the ISO-DH protocol:
+
+1. Mutual authentication
+2. Secrecy of the key ``k``
+3. Forward secrecy of the key ``k`` 
+  (as long as the private DH keys are secret, 
+  the key ``k`` does not leak)
+
+**Protocol Flow**
+
+```
+A -> B: {A, gx}                            msg1
+B -> A: {B, gy, sign({A; gx; gy}, privB)}  msg2
+A -> B: {sign({B; gx; gy}, privA)}         msg3
+```
+
+The model of the protocol is split into two
+parts. The first part is in the ``DY.Example.DH.Protocol.Total``
+module which contains all the code that does
+not depend on the trace, e.g., message definitions,
+cryptographic functions, and message encoding.
+The second part is in the ``DY.Example.DH.Protocol.Stateful`` 
+module, containing the logic that depends on the
+trace, e.g., state definitions, state encoding, and sending messages.
+
+Since the model is split into two parts, the proof is also
+split into the two modules ``DY.Example.DH.Protocol.Total.Proof``
+and ``DY.Example.DH.Protocol.Stateful.Proof``. The first
+module contains helper lemmas about the total functions 
+used in the stateful proof to prove that every
+stateful function fulfills the trace invariants.
+
+The two modules that are left are the ``DY.Example.DH.SecurityProperties``
+module and the ``DY.Example.DH.Debug`` module. The former
+defines and proves the security properties, and the latter generates 
+an example trace of an honest protocol run.
+
+## Check and Run the Model
+To verify the F* code you can call ``make`` from either this 
+directory or the repository's root directory.
+To run the ``DY.Example.DH.Debug`` module you have to
+execute ``make test`` from this directory.
